wip

code/experimental/pkcs/Spec/Hacl.PKCS11.Lemmas.fst
@@ -1,1 +1,19 @@
 module Hacl.PKCS11.Lemmas
+
+open FStar.Seq
+
+
+val lemmaFindLExistIfSome: #a: Type -> f: (a -> bool) -> s: seq a -> Lemma
+  (requires
+    (Some? (find_l f s)))
+  (ensures (exists (a: nat {a < Seq.length s}). f (index s a)))
+  (decreases (Seq.length s))
+
+
+let rec lemmaFindLExistIfSome #a f s = 
+  if length s = 0 then ()
+  else if length s = 1 then () 
+  else
+    if f (head s) then ()
+    else 
+      lemmaFindLExistIfSome f (tail s)
