code/experimental/pkcs/Spec/Hacl.PKCS11.Lib.fst
@@ -2,21 +2,6 @@ module Hacl.PKCS11.Lib
 
 open FStar.Seq
 
-(* It is the same function as in FStar.Seq.Properties -> to replace *)
-val for_all: #a: eqtype -> f: (a -> bool) -> s: seq a -> 
-  Tot (r: bool {r ==> (forall (i: nat {i < Seq.length s}). f (index s i))})
-    (decreases (Seq.length s))
-
-let rec for_all #a f s = 
-  admit();
-  match length s with 
-    | 0 -> true
-    | _ -> 
-      if f (head s) then
-	for_all f (tail s)
-      else 
-	false
-
 val for_all2: #a: eqtype -> #b: eqtype -> f: (a -> b -> bool) -> s: seq a -> s1: seq b {Seq.length s = Seq.length s1} -> 
   Tot bool (decreases (Seq.length s))
 
